theories/Impure.v
@@ -34,21 +34,21 @@ Generalizable All Variables.
 (** * Definition *)
 
 (** The [impure] monad is an inductive datatype with two parameters: the
-    effect [i] to be used, and the type [α] of the result of the computation.
+    effect [F] to be used, and the type [α] of the result of the computation.
     The fact that [impure] is inductive rather than co-inductive means it is not
     possible to describe infinite computations.  This also means it is possible
     to interpret impure computations within Coq, providing an operational
-    semantics for [i]. *)
+    semantics for [F]. *)
 
-Inductive freer (i : effect) (α : Type) : Type :=
-| local (x : α) : freer i α
-| request_then {β} (e : i β) (f : β -> freer i α) : freer i α.
+Inductive freer (F : effect) (α : Type) : Type :=
+| local (x : α) : freer F α
+| request_then {β} (e : F β) (f : β -> freer F α) : freer F α.
 
 #[deprecated(note="Name will change to `freer`.")]
 Notation impure := freer (only parsing).
 
-Arguments local [i α] (x).
-Arguments request_then [i α β] (e f).
+Arguments local [F α] (x).
+Arguments request_then [F α β] (e f).
 
 Register freer as freespec.core.impure.type.
 Register local as freespec.core.impure.local.
@@ -58,26 +58,27 @@ Declare Scope impure_scope.
 Bind Scope impure_scope with freer.
 Delimit Scope impure_scope with impure.
 
-HB.mixin Record isMonadImpure (i : effect) (M : UU0 -> UU0) of Monad M := {
-    request : i ~~> M ; 
-    impure_lift (N : monad) (l : i ~~> N) : M ~~> N ;
-    impure_lift_ret : forall (N : monad) (l : i ~~> N) X (x : X),
+HB.mixin Record isMonadImpure (F : effect) (M : UU0 -> UU0) of Monad M := {
+    request : F ~~> M ;
+    impure_lift (N : monad) (l : F ~~> N) : M ~~> N ;
+    impure_lift_ret : forall (N : monad) (l : F ~~> N) X (x : X),
         impure_lift N l X (ret X x) = @ret N X x;
-    impure_lift_bind : forall (N : monad) (l : i ~~> N) X Y m (f : X -> M Y), 
+    impure_lift_bind : forall (N : monad) (l : F ~~> N) X Y m
+        (f : X -> M Y),
         impure_lift N l Y (m >>= f) = (impure_lift N l X m) >>= (fun x => impure_lift N l Y (f x)) ;
-    impure_lift_request : forall (N : monad) (l : i ~~> N) X (fx : i X), 
+    impure_lift_request : forall (N : monad) (l : F ~~> N) X (fx : F X),
         impure_lift N l X (request X fx) = l X fx;
-    impure_lift_unique : forall (N : monad) (l : i ~~> N) (impure_lift' : M ~~> N),
+    impure_lift_unique : forall (N : monad) (l : F ~~> N) (impure_lift' : M ~~> N),
             (forall X (x : X), impure_lift' X (ret X x) = @ret N X x) ->
             (forall X Y (m : M X) (f : X -> M Y), impure_lift' Y (m >>= f) = (impure_lift' X m) >>= (fun x => impure_lift' Y (f x))) ->
-            (forall X (fx : i X), (impure_lift' X (request X fx)) = l X fx) ->
+            (forall X (fx : F X), (impure_lift' X (request X fx)) = l X fx) ->
         forall X (m : M X), impure_lift' X m = impure_lift N l X m
 }.
 
 
 #[short(type=impureMonad)]
-HB.structure Definition MonadImpure (i : effect) :=
-  {M of isMonadImpure i M & isMonad M & isFunctor M}.
+HB.structure Definition MonadImpure (F : effect) :=
+  {M of isMonadImpure F M & isMonad M & isFunctor M}.
 
 (** * Monad Instances *)
 
@@ -86,15 +87,15 @@ HB.structure Definition MonadImpure (i : effect) :=
 Module ImpureModule.
 Section freer.
 
-Variable i : UU0 -> UU0.
-Definition acto := fun X => @impure i X.
+Variable F : UU0 -> UU0.
+Definition acto := fun X => @impure F X.
 Notation FM := acto.
 
-Definition impure_pure {α} (x : α) : impure i α := local x.
+Definition impure_pure {α} (x : α) : impure F α := local x.
 
 Let ret : idfun ~~> FM := fun _ => impure_pure. 
 
-Fixpoint impure_bind {α β} (p : impure i α) (f : α -> impure i β) : impure i β :=
+Fixpoint impure_bind {α β} (p : impure F α) (f : α -> impure F β) : impure F β :=
   match p with
   | local x => f x
   | request_then Y e g => request_then e (fun x => impure_bind (g x) f)
@@ -135,10 +136,10 @@ HB.instance Definition _ := @isMonad_ret_bind.Build acto ret bind left_neutral r
 
     To complete these two monadic operations, we introduce the [request]
     function, whose purpose is to define an impure computation that uses a given
-    primitive [e] from an effect [i], and returns its result.  [request] does
-    not parameterize the [impure] monad with [i] directly, but rather with a
-    generic effect [ix].  [ix] is constrained with the [Provide] notation, so
-    that it has to provide at least [i]'s primitives.  *)
+    primitive [e] from an effect [F], and returns its result.  [request] does
+    not parameterize the [impure] monad with [F] directly, but rather with a
+    generic effect [Fx].  [Fx] is constrained with the [Provide] notation, so
+    that it has to provide at least [F]'s primitives.  *)
 
 End freer.
 End ImpureModule.
@@ -148,21 +149,21 @@ HB.export ImpureModule.
 Module Impure.
 Section freer.
 
-Variable i : effect.
+Variable F : effect.
 
-Local Notation M := (acto i).
+Local Notation M := (acto F).
 
-Definition request_effect : i ~~> acto i := fun α e =>
+Definition request_effect : F ~~> acto F := fun α e =>
   request_then (inj_p e) (fun x => local x).
 
-Definition lifter (M : monad) `(l : i ~~> M) : acto i ~~> M :=
-  fix aux a (p : acto i a) :=
+Definition lifter (M : monad) `(l : F ~~> M) : acto F ~~> M :=
+  fix aux a (p : acto F a) :=
     match p with
     | local x => Ret x
     | request_then Y e f => l _ e >>= fun x => aux a (f x)
     end.
 
-Let lifter_ret : forall (cm : monad) (lifter_effect : i ~~> cm) X (x : X),
+Let lifter_ret : forall (cm : monad) (lifter_effect : F ~~> cm) X (x : X),
         lifter lifter_effect (ret X x) = @hierarchy.ret cm X x.
 Proof.
   rewrite/=/lifter.
@@ -170,7 +171,8 @@ Proof.
 Qed.
 
 
-Let lifter_bind : forall (cm : monad) (lifter_effect : i ~~> cm) X Y m (f : X -> M Y), 
+Let lifter_bind : forall (cm : monad) (lifter_effect : F ~~> cm) X Y m
+    (f : X -> M Y),
         lifter lifter_effect (m >>= f) = ( lifter lifter_effect m) >>= (fun x => lifter lifter_effect (f x)) .
 Proof.
     move=>cm lifter_effect X Y m f.
@@ -181,17 +183,18 @@ Proof.
     exact/boolp.funext/H.
 Qed.
 
-Let lifter_trigger : forall (cm : monad) (lifter_effect : i ~~> cm) X (fx : i X), 
+Let lifter_trigger : forall (cm : monad) (lifter_effect : F ~~> cm)
+    X (fx : F X),
         lifter lifter_effect (request_effect fx) = lifter_effect X fx.
 Proof.
     move=>cm lifter_effect X fx.
     by rewrite /lifter /request_effect /= bindmret.
 Qed.
 
-Let lifter_unique : forall (cm : monad) (lifter_effect : i ~~> cm) (lifter' : M ~~> cm),
+Let lifter_unique : forall (cm : monad) (lifter_effect : F ~~> cm) (lifter' : M ~~> cm),
             (forall X (x : X), lifter' X (ret X x) = @hierarchy.ret cm X x) ->
             (forall X Y (m : M X) (f : X -> M Y), lifter' Y (m >>= f) = (lifter' X m) >>= (fun x => lifter' Y (f x))) ->
-            (forall X (fx : i X),
+            (forall X (fx : F X),
               lifter' X (request_effect fx) = lifter_effect X fx) ->
         forall X (m : M X), lifter' X m = lifter lifter_effect m.
 Proof.
@@ -203,7 +206,7 @@ Proof.
     by rewrite -dtrigger' -dbind' /request_effect.
 Qed.
 
-HB.instance Definition _ := isMonadImpure.Build i M 
+HB.instance Definition _ := isMonadImpure.Build F M
   lifter_ret 
   lifter_bind 
   lifter_trigger
@@ -213,8 +216,8 @@ End freer.
 End Impure.
 HB.export Impure.
 
-Lemma impure_lift_if : forall (i : effect) (M : impureMonad i) (cm : monad)
-    (lifter_effect : i ~~> cm) X (m m' : M X) b,
+Lemma impure_lift_if : forall (F : effect) (M : impureMonad F) (cm : monad)
+    (lifter_effect : F ~~> cm) X (m m' : M X) b,
         impure_lift cm lifter_effect X (if b then m else m') = if b then ( impure_lift cm lifter_effect X m) else ( impure_lift cm lifter_effect X m').
 Proof.
     by move=>? ? ? ? ? ? ?; case.
@@ -223,14 +226,14 @@ HB.export impure_lift_if.
 
 Module ImpSt.
   Section impstate.
-        Variable i : effect.
+        Variable F : effect.
         Variable S : UU0.
-Definition request_effect `{Provide ix i} {A} (e : i A) : acto ix A :=
+Definition request_effect `{Provide Fx F} {A} (e : F A) : acto Fx A :=
   request_then (inj_p e) (fun x => local x).
 
-  Let iget `{Provide i (STORE S)} : acto i S :=
+  Let iget `{Provide F (STORE S)} : acto F S :=
     request_effect (inj_p Get).
-  Let iput `{Provide i (STORE S)} (s : S) : acto i () :=
+  Let iput `{Provide F (STORE S)} (s : S) : acto F () :=
     request_effect (inj_p (Put s)).
 
 (** Note: there have been attempts to turn [request] into a typeclass
@@ -253,9 +256,10 @@ End ImpSt.
 (* HB.export ImpSt. *)
 
 Module ImpureFuns.
-Definition trigger  `{Provide ix i} {im : impureMonad ix} : ix ~~> im := fun a e => request a (inj_p e). 
-Definition iget {S} `{Provide i (STORE S)} {im : impureMonad i} : im S:= trigger (inj_p Get).
-Definition iput {S} `{Provide i (STORE S)} {im : impureMonad i} (s : S) : im unit:= trigger (inj_p (Put s)).
+Definition trigger `{Provide Fx F} {im : impureMonad Fx} : Fx ~~> im :=
+  fun a e => request a (inj_p e).
+Definition iget {S} `{Provide F (STORE S)} {im : impureMonad F} : im S:= trigger (inj_p Get).
+Definition iput {S} `{Provide F (STORE S)} {im : impureMonad F} (s : S) : im unit:= trigger (inj_p (Put s)).
 End ImpureFuns.
 
 HB.export ImpureFuns.
